Prove behavioral refinement for LDRF-RA

src/ldrfra/PFtoRA.v
@@ -30,8 +30,10 @@ Require Import JoinedView.
 
 Require Import PFStep.
 Require Import OrdStep.
-Require Import RAStep.
+Require Import Writes.
+Require Import WStep.
 Require Import Stable.
+Require Import PFtoAPFSim.
 Require Import APFtoRASim.
 Require Import PFtoRAThread.
 
@@ -52,12 +54,15 @@ Module PFtoRA.
 
     Definition wf_j := JConfiguration.wf.
 
-    Inductive wf_ra (rels: RelWrites.t) (c: Configuration.t): Prop :=
+    Inductive wf_ra (rels: Writes.t) (c: Configuration.t): Prop :=
     | wf_ra_intro
         (WF: Configuration.wf c)
+        (PROMISES: forall tid lang st lc
+                     (TH: IdentMap.find tid (Configuration.threads c) = Some (existT _ lang st, lc)),
+            OrdLocal.reserve_only L (Local.promises lc))
         (RELS: forall tid lang st lc
                  (TH: IdentMap.find tid (Configuration.threads c) = Some (existT _ lang st, lc)),
-            RelWrites.wf rels (Local.promises lc) (Configuration.memory c))
+            Writes.wf L rels (Configuration.memory c))
     .
 
     Lemma wf_pf_thread
@@ -87,11 +92,9 @@ Module PFtoRA.
           rels c tid lang st lc
           (WF: wf_ra rels c)
           (FIND: IdentMap.find tid (Configuration.threads c) = Some (existT _ lang st, lc)):
-      PFtoRAThread.wf_ra rels (Thread.mk _ st lc (Configuration.sc c) (Configuration.memory c)).
+      PFtoRAThread.wf_ra L rels (Thread.mk _ st lc (Configuration.sc c) (Configuration.memory c)).
     Proof.
       inv WF. inv WF0. inv WF.
-      hexploit THREADS; eauto. i.
-      hexploit RELS; eauto. i.
       econs; eauto.
     Qed.
 
@@ -114,30 +117,34 @@ Module PFtoRA.
     Qed.
 
     Lemma step_ra_future
+          ordr ordw
           e tid rels1 rels2 c1 c2
           (WF1: wf_ra rels1 c1)
-          (STEP: RAConfiguration.step L e tid rels1 rels2 c1 c2):
+          (ORD: Ordering.le Ordering.plain ordw)
+          (STEP: WConfiguration.step L ordr ordw e tid rels1 rels2 c1 c2):
       <<WF2: wf_ra rels2 c2>>.
     Proof.
-      exploit RAConfiguration.step_future; try eapply WF1; eauto. i. des.
+      exploit WConfiguration.step_future; try eapply WF1; eauto. i. des.
       inv STEP. ss.
-      assert (STEPS': RAThread.steps L rels1 rels2
-                                     (Thread.mk _ st1 lc1 (Configuration.sc c1) (Configuration.memory c1))
-                                     (Thread.mk _ st4 lc4 sc4 memory4)).
-      { exploit RAThread.tau_steps_steps;
-          try eapply RAThread.cancel_steps_tau_steps; try exact CANCELS. i.
-        exploit RAThread.opt_step_steps; try exact STEP0. i.
-        exploit RAThread.tau_steps_steps;
-          try eapply RAThread.reserve_steps_tau_steps; try exact RESERVES. i.
-        eapply RAThread.steps_trans; [eauto|].
-        eapply RAThread.steps_trans; eauto. }
+      assert (STEPS': WThread.steps L ordr ordw rels1 rels2
+                                    (Thread.mk _ st1 lc1 (Configuration.sc c1) (Configuration.memory c1))
+                                    (Thread.mk _ st4 lc4 sc4 memory4)).
+      { exploit WThread.tau_steps_steps;
+          try eapply WThread.cancel_steps_tau_steps; try exact CANCELS. i.
+        exploit WThread.opt_step_steps; try exact STEP0. i.
+        exploit WThread.tau_steps_steps;
+          try eapply WThread.reserve_steps_tau_steps; try exact RESERVES. i.
+        eapply WThread.steps_trans; [eauto|].
+        eapply WThread.steps_trans; eauto.
+      }
       exploit wf_ra_thread; eauto. i.
-      hexploit RAThread.steps_rels_wf; try exact STEPS'; try apply x1. s. i.
+      hexploit WThread.steps_writes_wf; try exact STEPS'; try apply x1; ss. i.
       econs; ss. i. Configuration.simplify; ss.
-      exploit wf_ra_thread; try eapply TH; eauto. i.
-      inv WF1. inv WF. inv WF0.
-      exploit DISJOINT; try exact n; eauto. i.
-      hexploit RAThread.steps_rels_disjoint; try exact x; eauto. apply x1.
+      - hexploit OrdThread.rtc_cancel_step_reserve_only; try eapply x1; eauto. i. des.
+        hexploit WThread.opt_step_ord_opt_step; eauto. i.
+        hexploit OrdThread.opt_step_reserve_only; try exact H1; eauto. i. des.
+        hexploit OrdThread.rtc_reserve_step_reserve_only; eauto.
+      - exploit wf_ra_thread; try eapply TH; eauto. i. apply x2.
     Qed.
 
     Lemma steps_pf_future
@@ -160,9 +167,11 @@ Module PFtoRA.
     Qed.
 
     Lemma steps_ra_future
+          ordr ordw
           rels1 rels2 c1 c2
           (WF1: wf_ra rels1 c1)
-          (STEPS: RAConfiguration.steps L rels1 rels2 c1 c2):
+          (ORD: Ordering.le Ordering.plain ordw)
+          (STEPS: WConfiguration.steps L ordr ordw rels1 rels2 c1 c2):
       <<WF2: wf_ra rels2 c2>>.
     Proof.
       revert WF1. induction STEPS; i; ss.
@@ -172,34 +181,48 @@ Module PFtoRA.
 
     (* sim *)
 
-    Inductive sim_thread_sl (views: Loc.t -> Time.t -> list View.t) (rels: RelWrites.t)
-              (sc_pf sc_j sc_ra: TimeMap.t) (mem_pf mem_j mem_ra: Memory.t):
-      forall (sl_pf sl_j sl_ra: {lang: language & Language.state lang} * Local.t), Prop :=
+    Inductive sim_thread_sl (views: Loc.t -> Time.t -> list View.t) (rels: Writes.t)
+              (sc_pf sc_j sc_apf sc_ra: TimeMap.t) (mem_pf mem_j mem_apf mem_ra: Memory.t):
+      forall (sl_pf sl_j sl_apf sl_ra: {lang: language & Language.state lang} * Local.t), Prop :=
     | sim_thread_sl_intro
-        lang st_pf lc_pf st_j lc_j st_ra lc_ra
+        lang st_pf lc_pf st_j lc_j st_apf lc_apf st_ra lc_ra
         (SIM: PFtoRAThread.sim_thread L views rels
                                       (Thread.mk lang st_pf lc_pf sc_pf mem_pf)
                                       (Thread.mk lang st_j lc_j sc_j mem_j)
+                                      (Thread.mk lang st_apf lc_apf sc_apf mem_apf)
                                       (Thread.mk lang st_ra lc_ra sc_ra mem_ra)):
-        sim_thread_sl views rels sc_pf sc_j sc_ra mem_pf mem_j mem_ra
-                      (existT _ lang st_pf, lc_pf) (existT _ lang st_j, lc_j) (existT _ lang st_ra, lc_ra)
+        sim_thread_sl views rels sc_pf sc_j sc_apf sc_ra mem_pf mem_j mem_apf mem_ra
+                      (existT _ lang st_pf, lc_pf) (existT _ lang st_j, lc_j)
+                      (existT _ lang st_apf, lc_apf) (existT _ lang st_ra, lc_ra)
     .
 
-    Inductive sim_conf (views: Loc.t -> Time.t -> list View.t) (rels: RelWrites.t):
-      forall (c_pf c_j c_ra: Configuration.t), Prop :=
+    Definition option_rel4 {A B C D} (P: A -> B -> C -> D -> Prop):
+      option A -> option B -> option C -> option D -> Prop :=
+      fun a b c d =>
+        match a, b, c, d with
+        | Some x, Some y, Some z, Some w => P x y z w
+        | None, None, None, None => True
+        | _, _, _, _ => False
+        end.
+
+    Inductive sim_conf (views: Loc.t -> Time.t -> list View.t) (rels: Writes.t):
+      forall (c_pf c_j c_apf c_ra: Configuration.t), Prop :=
     | sim_conf_intro
         ths_pf sc_pf mem_pf
         ths_j sc_j mem_j
+        ths_apf sc_apf mem_apf
         ths_ra sc_ra mem_ra
         (THS: forall tid,
-            option_rel3
-              (sim_thread_sl views rels sc_pf sc_j sc_ra mem_pf mem_j mem_ra)
+            option_rel4
+              (sim_thread_sl views rels sc_pf sc_j sc_apf sc_ra mem_pf mem_j mem_apf mem_ra)
               (IdentMap.find tid ths_pf)
               (IdentMap.find tid ths_j)
+              (IdentMap.find tid ths_apf)
               (IdentMap.find tid ths_ra)):
         sim_conf views rels
                  (Configuration.mk ths_pf sc_pf mem_pf)
                  (Configuration.mk ths_j sc_j mem_j)
+                 (Configuration.mk ths_apf sc_apf mem_apf)
                  (Configuration.mk ths_ra sc_ra mem_ra)
     .
 
@@ -229,12 +252,22 @@ Module PFtoRA.
     Lemma init_wf_ra syn:
       wf_ra [] (Configuration.init syn).
     Proof.
-      econs; eauto using Configuration.init_wf. i. ss.
+      econs; eauto using Configuration.init_wf; i; ss.
+      - unfold Threads.init in *.
+        rewrite IdentMap.Facts.map_o in *.
+        destruct (@UsualFMapPositive.UsualPositiveMap'.find
+                    (@sigT _ (@Language.syntax ProgramEvent.t)) tid syn); inv TH.
+        apply inj_pair2 in H1. subst. ss. ii.
+        rewrite Memory.bot_get in *. ss.
+      - econs; i; ss.
+        unfold Memory.get, Memory.init, Cell.get, Cell.init in *. ss.
+        apply DOMap.singleton_find_inv in GET. des. inv GET0. ss.
     Qed.
 
     Lemma init_sim_conf syn:
       sim_conf (fun _ => fun _ => []) []
-               (Configuration.init syn) (Configuration.init syn) (Configuration.init syn).
+               (Configuration.init syn) (Configuration.init syn)
+               (Configuration.init syn) (Configuration.init syn).
     Proof.
       econs; ss. i. unfold option_rel3.
       destruct (IdentMap.find tid (Threads.init syn)) as [[[lang st] lc]|] eqn:FIND; ss.
@@ -246,10 +279,11 @@ Module PFtoRA.
       econs. econs; ss.
       - econs; ss; try refl. econs; try refl. ii.
         rewrite Memory.bot_get. ss.
+      - econs; ss. econs; ss; eauto. i.
+        unfold Memory.get, Memory.init, Cell.get, Cell.init in *. ss.
+        apply DOMap.singleton_find_inv in GET. des. inv GET0. ss.
       - econs; ss.
-        + econs; ss.
-          * econs; ss. i. condtac; ss. refl.
-          * ii. rewrite Memory.bot_get in *. ss.
+        + econs; ss. econs; ss. i. condtac; ss. refl.
         + econs; ss; i.
           * unfold Memory.get, Memory.init, Cell.get, Cell.init in *. ss.
             apply DOMap.singleton_find_inv in GET_SRC. des. inv GET_SRC0.
@@ -269,21 +303,21 @@ Module PFtoRA.
     Qed.
 
     Lemma sim_conf_terminal
-          views rrels c_pf c_j c_ra
-          (SIM: sim_conf views rrels c_pf c_j c_ra)
+          views rrels c_pf c_j c_apf c_ra
+          (SIM: sim_conf views rrels c_pf c_j c_apf c_ra)
           (TERMINAL: Configuration.is_terminal c_pf):
       Configuration.is_terminal c_ra.
     Proof.
       ii. inv SIM. specialize (THS tid).
-      unfold option_rel3 in *. ss. des_ifs.
-      destruct p as [[]]. destruct p0 as [[]]. inv THS.
-      apply inj_pair2 in H7. apply inj_pair2 in H4. apply inj_pair2 in H1. subst.
-      inv SIM. inv SIM_JOINED. inv SIM_RA. ss.
-      apply inj_pair2 in H2. apply inj_pair2 in H6. subst.
+      unfold option_rel4 in *. ss. des_ifs.
+      destruct p as [[]], p0 as [[]], p1 as [[]]. inv THS.
+      apply inj_pair2 in H7, H4, H1, H10. subst.
+      inv SIM. inv SIM_JOINED. inv SIM_APF. inv SIM_RA. ss.
+      apply inj_pair2 in H2, H6. subst.
       exploit TERMINAL; eauto. i. des.
       split; ss.
       inv THREAD. econs.
-      inv LOCAL0. rewrite PROMISES0.
+      inv LOCAL1. rewrite PROMISES0.
       eapply JSim.sim_local_memory_bot; eauto.
     Qed.
 
@@ -291,179 +325,196 @@ Module PFtoRA.
     (* step *)
 
     Lemma sim_conf_step
-          views1 rels1 c1_pf c1_j c1_ra
+          views1 rels1 c1_pf c1_j c1_apf c1_ra
           tid e_pf c2_pf
-          (SIM1: sim_conf views1 rels1 c1_pf c1_j c1_ra)
+          (SIM1: sim_conf views1 rels1 c1_pf c1_j c1_apf c1_ra)
           (WF1_PF: wf_pf c1_pf)
           (WF1_J: wf_j views1 c1_j)
+          (WF1_APF: wf_ra rels1 c1_apf)
           (WF1_RA: wf_ra rels1 c1_ra)
           (STEP: PFConfiguration.step L e_pf tid c1_pf c2_pf):
-      (exists e_j c2_j views2 e_ra rels2 c2_ra,
+      (exists e_j c2_j e_apf c2_apf views2 e_ra rels2 c2_ra,
           (<<STEP_J: JConfiguration.single_step e_j tid c1_j c2_j views1 views2>>) /\
-          (<<STEP_RA: RAConfiguration.step L e_ra tid rels1 rels2 c1_ra c2_ra>>) /\
+          (<<STEP_APF: WConfiguration.step L Ordering.na Ordering.plain
+                                           e_apf tid rels1 rels2 c1_apf c2_apf>>) /\
+          (<<STEP_RA: WConfiguration.step L Ordering.acqrel Ordering.acqrel
+                                          e_ra tid rels1 rels2 c1_ra c2_ra>>) /\
           (<<EVENT_J: JSim.sim_event e_j e_pf>>) /\
-          (<<EVENT_RA: APFtoRASim.sim_event e_ra e_j>>) /\
-          (<<SIM2: sim_conf views2 rels2 c2_pf c2_j c2_ra>>)) \/
-      (<<RACE: RARaceW.ra_race_steps L rels1 c1_ra>>).
+          (<<EVENT_APF: PFtoAPFSim.sim_event e_apf e_j>>) /\
+          (<<EVENT_RA: APFtoRASim.sim_event e_ra e_apf>>) /\
+          (<<SIM2: sim_conf views2 rels2 c2_pf c2_j c2_apf c2_ra>>)) \/
+      (<<RACE: RARaceW.ra_race_steps L Ordering.acqrel Ordering.acqrel rels1 c1_ra>>).
     Proof.
       dup SIM1. inv SIM0. inv STEP. ss.
-      dup THS. specialize (THS0 tid). unfold option_rel3 in THS0. des_ifs.
+      dup THS. specialize (THS0 tid). unfold option_rel4 in THS0. des_ifs. 
       inv THS0. apply inj_pair2 in H1. subst.
       exploit wf_pf_thread; eauto. s. i.
       exploit wf_j_thread; eauto. s. i.
-      exploit wf_ra_thread; eauto. s. i.
+      exploit wf_ra_thread; try exact WF1_APF; eauto. s. i.
+      exploit wf_ra_thread; try exact WF1_RA; eauto. s. i.
       exploit PFtoRAThread.sim_thread_cancel_steps; eauto.
       { exploit PFtoRAThread.cancel_steps_pf_future; eauto. i.
         exploit PFtoRAThread.opt_step_pf_future; eauto. i.
         exploit PFtoRAThread.reserve_steps_pf_future; eauto. i.
-        destruct (classic (e_pf = ThreadEvent.failure)).
-        - subst. inv STEP0. inv STEP; inv STEP0. inv LOCAL. inv LOCAL0. ss.
-        - eapply opt_step_promise_consistent; eauto; try apply x3.
+        destruct (classic (ThreadEvent.get_machine_event e_pf = MachineEvent.failure)).
+        - inv STEP0; ss. inv STEP; inv STEP0; ss.
+          inv LOCAL; ss; inv LOCAL0; ss.
+        - eapply opt_step_promise_consistent; eauto; try apply x4.
           eapply rtc_reserve_step_promise_consistent; eauto.
           eapply consistent_promise_consistent;
-            try eapply PF.pf_consistent_consistent; eauto; try apply x5.
+            try eapply PF.pf_consistent_consistent; eauto; try apply x6.
       }
       i. des.
       exploit PFtoRAThread.cancel_steps_pf_future; eauto. i.
       exploit PFtoRAThread.cancel_steps_j_future; eauto. i.
-      exploit PFtoRAThread.cancel_steps_ra_future; eauto. i.
+      exploit PFtoRAThread.cancel_steps_ra_future; try exact x2; eauto. i.
+      exploit PFtoRAThread.cancel_steps_ra_future; try exact x3; eauto. i.
       exploit PFtoRAThread.sim_thread_opt_step; eauto.
       { exploit PFtoRAThread.opt_step_pf_future; eauto. i.
         exploit PFtoRAThread.reserve_steps_pf_future; eauto. i.
-        destruct (classic (e_pf = ThreadEvent.failure)).
-        - subst. inv STEP0. inv STEP; inv STEP0. inv LOCAL. inv LOCAL0. ss.
+        destruct (classic (ThreadEvent.get_machine_event e_pf = MachineEvent.failure)).
+        - inv STEP0; ss. inv STEP; inv STEP0; ss.
+          inv LOCAL; ss; inv LOCAL0; ss.
         - eapply rtc_reserve_step_promise_consistent; eauto.
           eapply consistent_promise_consistent;
-            try eapply PF.pf_consistent_consistent; eauto; try apply x7.
+            try eapply PF.pf_consistent_consistent; eauto; try apply x9.
       }
       i. des; cycle 1.
       { right. unfold RARaceW.ra_race_steps.
         esplits; [econs 1|..]; eauto. s.
-        eapply RAThread.tau_steps_steps.
-        eapply RAThread.cancel_steps_tau_steps; eauto. }
+        eapply WThread.tau_steps_steps.
+        eapply WThread.cancel_steps_tau_steps; eauto.
+      }
       exploit PFtoRAThread.opt_step_pf_future; eauto. i.
       exploit PFtoRAThread.opt_step_j_future; eauto. i.
-      exploit PFtoRAThread.opt_step_ra_future; eauto. i.
+      exploit PFtoRAThread.opt_step_ra_future; try exact x6; eauto; ss. i.
+      exploit PFtoRAThread.opt_step_ra_future; try exact x7; eauto; ss. i.
       exploit PFtoRAThread.sim_thread_reserve_steps; eauto.
-      { exploit PFtoRAThread.reserve_steps_pf_future; eauto. i.
-        destruct (classic (e_pf = ThreadEvent.failure)).
-        - subst. inv STEP0. inv STEP; inv STEP0. inv LOCAL. inv LOCAL0.
-          eapply rtc_reserve_step_promise_consistent2; eauto. ss.
-        - eapply consistent_promise_consistent;
-            try eapply PF.pf_consistent_consistent; eauto; try apply x9.
+      { exploit PFtoRAThread.reserve_steps_pf_future; eauto. s. i.
+        destruct (classic (ThreadEvent.get_machine_event e_pf = MachineEvent.failure)).
+        - hexploit rtc_reserve_step_promise_consistent2; eauto.
+          inv STEP0; ss. inv STEP; inv STEP0; ss.
+          inv LOCAL; ss; inv LOCAL0; ss.
+        - hexploit consistent_promise_consistent;
+            try eapply PF.pf_consistent_consistent; eauto; try apply x12.
       }
       i. des.
       exploit PFtoRAThread.reserve_steps_pf_future; eauto. i.
       exploit PFtoRAThread.reserve_steps_j_future; eauto. i.
-      exploit PFtoRAThread.reserve_steps_ra_future; eauto. i.
-      assert (STEPS': RAThread.steps L rels1 rels2 (Thread.mk _ st_ra lc_ra sc_ra mem_ra) e2_ra1).
-      { exploit RAThread.tau_steps_steps;
-          try eapply RAThread.cancel_steps_tau_steps; try exact STEP_RA. i.
-        exploit RAThread.opt_step_steps; eauto. i.
-        exploit RAThread.tau_steps_steps;
-          try eapply RAThread.reserve_steps_tau_steps; try exact STEP_RA1. i.
-        eapply RAThread.steps_trans; eauto.
-        eapply RAThread.steps_trans; eauto. }
+      exploit PFtoRAThread.reserve_steps_ra_future; try exact x10; eauto. i.
+      exploit PFtoRAThread.reserve_steps_ra_future; try exact x11; eauto. i.
+      assert (STEPS': WThread.steps L Ordering.acqrel Ordering.acqrel
+                                    rels1 rels2 (Thread.mk _ st_ra lc_ra sc_ra mem_ra) e2_ra1).
+      { exploit WThread.tau_steps_steps;
+          try eapply WThread.cancel_steps_tau_steps; try exact STEP_RA. i.
+        exploit WThread.opt_step_steps; eauto. i.
+        exploit WThread.tau_steps_steps;
+          try eapply WThread.reserve_steps_tau_steps; try exact STEP_RA1. i.
+        eapply WThread.steps_trans; eauto.
+        eapply WThread.steps_trans; eauto.
+      }
 
-      destruct (classic (e_pf = ThreadEvent.failure)).
-      { subst. inv EVENT_J. inv EVENT_RA.
-        destruct e2_j1 as [st4_j lc4_j sc4_j mem4_j], e2_ra1 as [st4_ra lc4_ra sc4_ra mem4_ra].
+      destruct (classic (ThreadEvent.get_machine_event e_pf = MachineEvent.failure)).
+      { destruct e2_j1 as [st4_j lc4_j sc4_j mem4_j],
+                 e2_apf1 as [st4_apf lc4_apf sc4_apf mem4_apf],
+                 e2_ra1 as [st4_ra lc4_ra sc4_ra mem4_ra].
         left. esplits.
-        - econs; eauto. ss.
-        - econs; eauto. ss.
+        - econs; eauto. inv EVENT_J; ss.
+        - econs; eauto. inv EVENT_J; inv EVENT_APF; ss.
+        - econs; eauto. inv EVENT_J; inv EVENT_APF; inv EVENT_RA; ss.
         - ss.
-        - econs.
+        - ss.
+        - ss.
         - econs; ss. i.
           repeat rewrite IdentMap.gsspec. condtac; ss.
-          specialize (THS tid0). unfold option_rel3 in THS. des_ifs. inv THS. ss.
+          specialize (THS tid0). unfold option_rel4 in THS. des_ifs. inv THS. ss.
           inv SIM4. ss. econs. econs; s; eauto; try apply SIM3.
           * inv SIM_JOINED.
-            apply inj_pair2 in H2. apply inj_pair2 in H6. subst.
+            apply inj_pair2 in H3, H7. subst.
             econs; s; eauto; try by (inv SIM3; inv SIM_JOINED; ss).
             exploit JThread.rtc_cancel_step_future; eauto; try apply x1. s. i. des.
             exploit JThread.opt_step_future; eauto; try apply x1. s. i. des.
             exploit JThread.rtc_reserve_step_future; eauto. s. i. des.
             eapply JSim.sim_local_le; try exact LOCAL.
             etrans; eauto. refl.
+          * inv SIM_APF. ss. subst.
+            econs; s; eauto; try by (inv SIM3; inv SIM_APF; ss).
           * inv SIM_RA. ss. subst.
             econs; s; eauto; try by (inv SIM3; inv SIM_RA; ss).
-            inv LOCAL. econs; ss. i.
-            exploit wf_ra_thread; try exact WF1_RA; try eapply Heq4. s. i.
-            eapply RAThread.steps_rels_disjoint; try exact STEPS'; ss; try apply x2; try apply x12.
-            inv WF1_RA. inv WF. inv WF0. ss.
-            eapply DISJOINT; [|eapply Heq1|eapply Heq4]. congr.
-          * econs; try apply SIM3; try apply NORMAL_J.
+          * econs; try apply SIM3; try apply NORMAL_APF.
           * econs; try apply SIM3; try apply NORMAL_RA.
           * econs; s; try apply SIM3; try apply STABLE_RA.
-            exploit RAThread.steps_future; try exact STEPS'; try apply x2. s. i. des.
-            exploit wf_ra_thread; try exact WF1_RA; try eapply Heq4. s. i.
-            exploit Stable.future_stable_tview; try eapply STABLE_RA; try apply x12; eauto.
+            exploit WThread.steps_future; try exact STEPS'; try apply x3. s. i. des.
+            exploit wf_ra_thread; try exact WF1_RA; try eapply Heq6. s. i.
+            exploit Stable.future_stable_tview; try eapply STABLE_RA; try apply x16; eauto.
       }
 
       exploit PFtoRAThread.sim_thread_consistent; try eapply CONSISTENT; eauto. i. des; cycle 1.
       { right. unfold RARaceW.ra_race_steps.
         esplits; [econs 1|..]; try eapply RACE; eauto. s.
-        eapply RAThread.steps_trans; eauto.
-        eapply RAThread.tau_steps_steps; eauto. }
-      destruct e2_j1 as [st4_j lc4_j sc4_j mem4_j], e2_ra1 as [st4_ra lc4_ra sc4_ra mem4_ra].
+        eapply WThread.steps_trans; eauto.
+        eapply WThread.tau_steps_steps; eauto.
+      }
+      destruct e2_j1 as [st4_j lc4_j sc4_j mem4_j],
+               e2_apf1 as [st4_apf lc4_apf sc4_apf mem4_apf],
+               e2_ra1 as [st4_ra lc4_ra sc4_ra mem4_ra].
       left. esplits.
       - econs; eauto.
       - econs; eauto.
+      - econs; eauto.
+      - ss.
       - ss.
       - ss.
       - econs; ss. i.
         repeat rewrite IdentMap.gsspec. condtac; ss.
-        specialize (THS tid0). unfold option_rel3 in THS. des_ifs. inv THS. ss.
+        specialize (THS tid0). unfold option_rel4 in THS. des_ifs. inv THS. ss.
         inv SIM4. ss. econs. econs; s; eauto; try apply SIM3.
         * inv SIM_JOINED.
-          apply inj_pair2 in H3. apply inj_pair2 in H7. subst.
+          apply inj_pair2 in H3, H7. subst.
           econs; s; eauto; try by (inv SIM3; inv SIM_JOINED; ss).
           exploit JThread.rtc_cancel_step_future; eauto; try apply x1. s. i. des.
           exploit JThread.opt_step_future; eauto; try apply x1. s. i. des.
           exploit JThread.rtc_reserve_step_future; eauto. s. i. des.
           eapply JSim.sim_local_le; try exact LOCAL.
           etrans; eauto. refl.
+        * inv SIM_APF. ss. subst.
+          econs; s; eauto; try by (inv SIM3; inv SIM_APF; ss).
         * inv SIM_RA. ss. subst.
           econs; s; eauto; try by (inv SIM3; inv SIM_RA; ss).
-          inv LOCAL. econs; ss. i.
-          exploit wf_ra_thread; try exact WF1_RA; try eapply Heq4. s. i.
-          eapply RAThread.steps_rels_disjoint; try exact STEPS'; ss; try apply x2; try apply x12.
-          inv WF1_RA. inv WF. inv WF0. ss.
-          eapply DISJOINT; [|eapply Heq1|eapply Heq4]. congr.
-        * econs; try apply SIM3; try apply NORMAL_J.
+        * econs; try apply SIM3; try apply NORMAL_APF.
         * econs; try apply SIM3; try apply NORMAL_RA.
         * econs; s; try apply SIM3; try apply STABLE_RA.
-          exploit RAThread.steps_future; try exact STEPS'; try apply x2. s. i. des.
-          exploit wf_ra_thread; try exact WF1_RA; try eapply Heq4. s. i.
-          exploit Stable.future_stable_tview; try eapply STABLE_RA; try apply x12; eauto.
+          exploit WThread.steps_future; try exact STEPS'; try apply x3. s. i. des.
+          exploit wf_ra_thread; try exact WF1_RA; try eapply Heq6. s. i.
+          exploit Stable.future_stable_tview; try eapply STABLE_RA; try apply x16; eauto.
     Qed.
 
     Lemma sim_conf_steps
-          views1 rels1 c1_pf c1_j c1_ra
+          views1 rels1 c1_pf c1_j c1_apf c1_ra
           c2_pf
-          (SIM1: sim_conf views1 rels1 c1_pf c1_j c1_ra)
+          (SIM1: sim_conf views1 rels1 c1_pf c1_j c1_apf c1_ra)
           (WF1_PF: wf_pf c1_pf)
           (WF1_J: wf_j views1 c1_j)
+          (WF1_APF: wf_ra rels1 c1_apf)
           (WF1_RA: wf_ra rels1 c1_ra)
           (STEPS: rtc (PFConfiguration.all_step L) c1_pf c2_pf):
-      (exists c2_j views2 rels2 c2_ra,
-          (<<STEPS_RA: RAConfiguration.steps L rels1 rels2 c1_ra c2_ra>>) /\
+      (exists c2_j c2_apf views2 rels2 c2_ra,
           (<<STEPS_J: JConfiguration.single_steps c1_j c2_j views1 views2>>) /\
-          (<<SIM2: sim_conf views2 rels2 c2_pf c2_j c2_ra>>)) \/
-      (<<RACE: RARaceW.ra_race_steps L rels1 c1_ra>>).
+          (<<STEPS_APF: WConfiguration.steps L Ordering.na Ordering.plain rels1 rels2 c1_apf c2_apf>>) /\
+          (<<STEPS_RA: WConfiguration.steps L Ordering.acqrel Ordering.acqrel rels1 rels2 c1_ra c2_ra>>) /\
+          (<<SIM2: sim_conf views2 rels2 c2_pf c2_j c2_apf c2_ra>>)) \/
+      (<<RACE: RARaceW.ra_race_steps L Ordering.acqrel Ordering.acqrel rels1 c1_ra>>).
     Proof.
-      revert views1 rels1 c1_j c1_ra SIM1 WF1_PF WF1_J WF1_RA.
+      revert views1 rels1 c1_j c1_apf c1_ra SIM1 WF1_PF WF1_J WF1_APF WF1_RA.
       induction STEPS; i.
       { left. esplits; try by econs 1. ss. }
       inv H. exploit sim_conf_step; eauto. i. des; eauto.
       exploit step_pf_future; eauto. i. des.
       exploit step_j_future; eauto. i. des.
-      exploit step_ra_future; eauto. i. des.
+      exploit step_ra_future; try exact STEP_APF; eauto. i. des.
+      exploit step_ra_future; try exact STEP_RA; eauto. i. des.
       exploit IHSTEPS; eauto. i. des.
-      - left. esplits.
-        + econs 2; eauto.
-        + econs 2; eauto.
-        + ss.
+      - left. esplits; (try by econs 2; eauto); ss.
       - right. unfold RARaceW.ra_race_steps in *. des.
         esplits; [econs 2; eauto|..]; eauto.
     Qed.
@@ -472,139 +523,165 @@ Module PFtoRA.
     (* racefree *)
 
     Lemma sim_conf_racy_read
-          views1 rels1 c1_pf c1_j c1_ra
+          views1 rels1 c1_pf c1_j c1_apf c1_ra
           loc ts e_pf tid c2_pf
-          (SIM1: sim_conf views1 rels1 c1_pf c1_j c1_ra)
+          (SIM1: sim_conf views1 rels1 c1_pf c1_j c1_apf c1_ra)
           (WF1_PF: wf_pf c1_pf)
           (WF1_J: wf_j views1 c1_j)
+          (WF1_APF: wf_ra rels1 c1_apf)
           (WF1_RA: wf_ra rels1 c1_ra)
           (STEP: PFRace.racy_read_step L loc ts e_pf tid c1_pf c2_pf)
           (LOC: L loc)
-          (RELS: ~ List.In (loc, ts) rels1):
-      (<<RACE: RARaceW.ra_race_steps L rels1 c1_ra>>).
+          (RELS: exists ord, List.In (loc, ts, ord) rels1 /\ Ordering.le ord Ordering.strong_relaxed):
+      (<<RACE: RARaceW.ra_race_steps L Ordering.acqrel Ordering.acqrel rels1 c1_ra>>).
     Proof.
       inv STEP. inv SIM1. ss.
-      specialize (THS tid). unfold option_rel3 in THS. des_ifs.
+      specialize (THS tid). unfold option_rel4 in THS. des_ifs.
       inv THS. apply inj_pair2 in H1. subst.
       exploit wf_pf_thread; eauto. s. i.
       exploit wf_j_thread; eauto. s. i.
-      exploit wf_ra_thread; eauto. s. i.
+      exploit wf_ra_thread; try exact WF1_APF; eauto. s. i.
+      exploit wf_ra_thread; try exact WF1_RA; eauto. s. i.
       exploit PFtoRAThread.sim_thread_cancel_steps; eauto.
-      { destruct (classic (e_pf = ThreadEvent.failure)).
-        - subst. inv STEP0; inv STEP; inv STEP0. inv LOCAL. inv LOCAL0. ss.
+      { destruct (classic (ThreadEvent.get_machine_event e_pf = MachineEvent.failure)).
+        - inv STEP0; ss. inv STEP; inv STEP0; ss. inv LOCAL; ss; inv LOCAL0; ss.
         - exploit PFtoRAThread.cancel_steps_pf_future; eauto. i.
           exploit PFtoRAThread.opt_step_pf_future; eauto. i.
           exploit PFtoRAThread.reserve_steps_pf_future; eauto. i.
-          eapply opt_step_promise_consistent; eauto; try eapply x3.
+          eapply opt_step_promise_consistent; eauto; try eapply x4.
           eapply rtc_reserve_step_promise_consistent; eauto.
           eapply consistent_promise_consistent; try eapply PF.pf_consistent_consistent;
-            try eapply CONSISTENT; try eapply x5; eauto.
+            try eapply CONSISTENT; try eapply x6; eauto.
       }
       i. des.
       exploit PFtoRAThread.cancel_steps_pf_future; try eapply x0; eauto. i.
       exploit PFtoRAThread.cancel_steps_j_future; try eapply x1; eauto. i.
       exploit PFtoRAThread.cancel_steps_ra_future; try eapply x2; eauto. i.
+      exploit PFtoRAThread.cancel_steps_ra_future; try eapply x3; eauto. i.
       exploit PFtoRAThread.sim_thread_opt_step; eauto.
-      { destruct (classic (e_pf = ThreadEvent.failure)).
-        - subst. inv STEP0; inv STEP; inv STEP0. inv LOCAL. inv LOCAL0. ss.
+      { destruct (classic (ThreadEvent.get_machine_event e_pf = MachineEvent.failure)).
+        - inv STEP0; ss. inv STEP; inv STEP0; ss. inv LOCAL; ss; inv LOCAL0; ss.
         - exploit PFtoRAThread.opt_step_pf_future; eauto. i.
           exploit PFtoRAThread.reserve_steps_pf_future; eauto. i.
           eapply rtc_reserve_step_promise_consistent; eauto.
           eapply consistent_promise_consistent; try eapply PF.pf_consistent_consistent;
-            try eapply CONSISTENT; try eapply x7; eauto.
+            try eapply CONSISTENT; try eapply x9; eauto.
       }
       i. unfold RARaceW.ra_race_steps. des; cycle 1.
       { esplits; [econs 1|..]; eauto. s.
-        eapply RAThread.tau_steps_steps; eapply RAThread.cancel_steps_tau_steps; eauto. }
-      hexploit APFtoRASim.sim_local_promise_consistent; try eapply SIM2.
+        eapply WThread.tau_steps_steps; eapply WThread.cancel_steps_tau_steps; eauto.
+      }
+      hexploit PFtoAPFSim.sim_thread_promise_consistent; try eapply SIM2; i.
       { inv SIM2. inv SIM_JOINED.
-        apply inj_pair2 in H2. apply inj_pair2 in  H3. subst. ss.
+        apply inj_pair2 in H2, H3. subst. ss.
         eapply JSim.sim_local_promise_consistent; eauto.
         exploit PFtoRAThread.reserve_steps_pf_future; eauto. i.
-        destruct (classic (e_pf = ThreadEvent.failure)).
-        - subst. inv STEP0; inv STEP; inv STEP0. inv LOCAL0. inv LOCAL1. ss.
+        destruct (classic (ThreadEvent.get_machine_event e_pf = MachineEvent.failure)).
+        - inv STEP0; ss. inv STEP; inv STEP0; ss. inv LOCAL0; ss; inv LOCAL1; ss.
         - exploit PFtoRAThread.opt_step_pf_future; eauto. i. des.
           exploit PFtoRAThread.reserve_steps_pf_future; eauto. i.
           hexploit consistent_promise_consistent; try eapply PF.pf_consistent_consistent;
-            try eapply CONSISTENT; try eapply x8; eauto. s. i.
+            try eapply CONSISTENT; try eapply x10; eauto. s. i.
           hexploit rtc_reserve_step_promise_consistent; try exact H1; eauto. i.
-          hexploit opt_step_promise_consistent; try eapply x6; eauto.
+          hexploit opt_step_promise_consistent; try eapply x8; eauto.
       }
-      i. inv READ; inv EVENT_J; inv EVENT_RA; ss.
-      - inv STEP_RA0. esplits; [econs 1|..]; eauto; ss.
-        + eapply RAThread.tau_steps_steps; eapply RAThread.cancel_steps_tau_steps; eauto.
-        + unfold RARaceW.ra_race. splits; eauto.
-          inv SIM2. inv SIM_JOINED. inv SIM_RA.
-          apply inj_pair2 in H3. apply inj_pair2 in H4. subst. ss.
-          inv LOCAL0. inv TVIEW. rewrite CUR.
+      hexploit APFtoRASim.sim_local_promise_consistent; try eapply SIM2; eauto. i.
+      inv READ; inv EVENT_J; inv EVENT_APF; inv EVENT_RA; ss.
+      - inv STEP_RA0. inv STEP; ss. inv STEP1; inv STEP; ss. inv LOCAL; ss.
+        esplits; [econs 1|..].
+        + eauto.
+        + eapply WThread.tau_steps_steps; eapply WThread.cancel_steps_tau_steps; eauto.
+        + ss.
+        + eauto.
+        + unfold RARaceW.ra_race.
+          left. esplits; eauto; ss.
+          inv SIM2. inv SIM_JOINED. inv SIM_APF. inv SIM_RA. ss.
+          apply inj_pair2 in H4, H5. subst. ss.
+          unfold RARaceW.wr_race.
+          inv LOCAL2. inv TVIEW. rewrite CUR.
+          esplits; eauto.
           eapply TimeFacts.le_lt_lt; eauto. condtac.
           * inv LOCAL. inv TVIEW. inv CUR0. apply RLX.
           * inv LOCAL. inv TVIEW. inv CUR0.
-            inv NORMAL_J. inv NORMAL_TVIEW. ss. rewrite CUR0; ss.
-      - inv STEP_RA0. esplits; [econs 1|..]; eauto; ss.
-        + eapply RAThread.tau_steps_steps; eapply RAThread.cancel_steps_tau_steps; eauto.
-        + unfold RARaceW.ra_race. splits; eauto.
-          inv SIM2. inv SIM_JOINED. inv SIM_RA.
-          apply inj_pair2 in H3. apply inj_pair2 in H4. subst. ss.
-          inv LOCAL0. inv TVIEW. rewrite CUR.
+            inv NORMAL_APF. inv NORMAL_TVIEW. ss.
+            destruct e2_apf; ss. subst. ss.
+            rewrite CUR0; ss.
+      - inv STEP_RA0. inv STEP; ss. inv STEP1; inv STEP; ss. inv LOCAL; ss.
+        esplits; [econs 1|..].
+        + eauto.
+        + eapply WThread.tau_steps_steps; eapply WThread.cancel_steps_tau_steps; eauto.
+        + ss.
+        + eauto.
+        + unfold RARaceW.ra_race.
+          left. esplits; eauto; ss.
+          inv SIM2. inv SIM_JOINED. inv SIM_APF. inv SIM_RA. ss.
+          apply inj_pair2 in H4, H5. subst. ss.
+          unfold RARaceW.wr_race.
+          inv LOCAL3. inv TVIEW. rewrite CUR.
+          esplits; eauto.
           eapply TimeFacts.le_lt_lt; eauto. condtac.
           * inv LOCAL. inv TVIEW. inv CUR0. apply RLX.
           * inv LOCAL. inv TVIEW. inv CUR0.
-            inv NORMAL_J. inv NORMAL_TVIEW. ss. rewrite CUR0; ss.
+            inv NORMAL_APF. inv NORMAL_TVIEW. ss.
+            destruct e2_apf; ss. subst. ss.
+            rewrite CUR0; ss.
     Qed.
 
     Lemma sim_conf_racefree
-          views rels c_pf c_j c_ra
-          (SIM: sim_conf views rels c_pf c_j c_ra)
+          views rels c_pf c_j c_apf c_ra
+          (SIM: sim_conf views rels c_pf c_j c_apf c_ra)
           (WF_PF: wf_pf c_pf)
           (WF_J: wf_j views c_j)
+          (WF_APF: wf_ra rels c_apf)
           (WF_RA: wf_ra rels c_ra)
-          (RA_RACEFREE: RARaceW.racefree L rels c_ra):
+          (RA_RACEFREE: RARaceW.racefree L Ordering.acqrel Ordering.acqrel rels c_ra):
       PFRace.racefree_view L c_pf.
     Proof.
       ii. exploit sim_conf_steps; eauto. i. des; cycle 1.
       { unfold RARaceW.ra_race_steps in *. des. eauto. }
       exploit steps_pf_future; eauto. i. des.
       exploit steps_j_future; eauto. i. des.
-      exploit steps_ra_future; eauto. i. des.
+      exploit steps_ra_future; try exact WF_APF; eauto; ss. i. des.
+      exploit steps_ra_future; try exact WF_RA; eauto; ss. i. des.
       inv WRITE.
       exploit sim_conf_step; try exact STEP; eauto. i. des; cycle 1.
       { unfold RARaceW.ra_race_steps in *. des.
         eapply RA_RACEFREE; cycle 1; eauto.
-        eapply RAConfiguration.steps_trans; eauto. }
-      assert (WRITE_RA: ~ List.In (loc, ts) rels0).
-      { inv WRITE0; inv EVENT_J; inv EVENT_RA; ss.
-        - hexploit RAConfiguration.write_rels; try exact STEP_RA; try eapply x2; ss. i.
-          inv STEP_RA. inv STEP0; ss. inv STEP1.
-          unfold RelWrites.append. ss. condtac; ss. condtac; ss.
-          destruct ordw; ss.
-        - hexploit RAConfiguration.write_rels; try exact STEP_RA; try eapply x2; ss. i.
-          inv STEP_RA. inv STEP0; ss. inv STEP1.
-          unfold RelWrites.append. ss. condtac; ss. condtac; ss.
-          destruct ordw; ss.
+        eapply WConfiguration.steps_trans; eauto.
+      }
+      assert (WRITE_RA: exists ord, List.In (loc, ts, ord) rels0 /\ Ordering.le ord Ordering.strong_relaxed).
+      { inv WRITE0; inv EVENT_J; inv EVENT_APF; inv EVENT_RA; ss.
+        - inv STEP_APF. ss. inv STEP0; ss. inv STEP1.
+          unfold Writes.append. ss. condtac; ss.
+          esplits; [left|]; eauto.
+        - inv STEP_APF. ss. inv STEP0; ss. inv STEP1.
+          unfold Writes.append. ss. condtac; ss.
+          esplits; [left|]; eauto.
       }
       exploit step_pf_future; try exact STEP; eauto. i. des.
       exploit step_j_future; try exact STEP_J; eauto. i. des.
+      exploit step_ra_future; try exact STEP_APF; eauto. i. des.
       exploit step_ra_future; try exact STEP_RA; eauto. i. des.
       exploit sim_conf_steps; try exact CSTEPS2; eauto. i. des; cycle 1.
       { unfold RARaceW.ra_race_steps in *. des.
         eapply RA_RACEFREE; cycle 1; eauto.
-        eapply RAConfiguration.steps_trans; [eauto|].
-        econs 2; eauto. }
+        eapply WConfiguration.steps_trans; [eauto|].
+        econs 2; eauto.
+      }
       exploit steps_pf_future; try exact CSTEPS2; eauto. i. des.
       exploit steps_j_future; try exact STEPS_J0; eauto. i. des.
+      exploit steps_ra_future; try exact STEPS_APF0; eauto. i. des.
       exploit steps_ra_future; try exact STEPS_RA0; eauto. i. des.
-      assert (READ_RA: ~ List.In (loc, ts) rels1).
-      { inv WRITE0; inv EVENT_J; inv EVENT_RA; ss.
-        - exploit RAConfiguration.write_get_None; try exact STEP_RA; ss; try apply x2. i. des.
-          eapply RAConfiguration.steps_rels; eauto.
-        - exploit RAConfiguration.write_get_None; try exact STEP_RA; ss; try apply x2. i. des.
-          eapply RAConfiguration.steps_rels; eauto.
+      assert (READ_RA: exists ord, List.In (loc, ts, ord) rels1 /\ Ordering.le ord Ordering.strong_relaxed).
+      { exploit WConfiguration.steps_rels_incl; try exact STEPS_APF0. i. des. subst.
+        esplits.
+        - apply List.in_or_app. right. eauto.
+        - ss.
       }
       exploit sim_conf_racy_read; eauto. unfold RARaceW.ra_race_steps. i. des.
       eapply RA_RACEFREE; cycle 1; eauto.
-      eapply RAConfiguration.steps_trans; eauto.
-      eapply RAConfiguration.steps_trans; eauto.
+      eapply WConfiguration.steps_trans; eauto.
+      eapply WConfiguration.steps_trans; eauto.
       econs 2; eauto.
     Qed.
 
@@ -612,49 +689,53 @@ Module PFtoRA.
     (* behaviors *)
 
     Lemma sim_conf_behavior
-          views rels c_pf c_j c_ra
-          (SIM: sim_conf views rels c_pf c_j c_ra)
+          views rels c_pf c_j c_apf c_ra
+          (SIM: sim_conf views rels c_pf c_j c_apf c_ra)
           (WF_PF: wf_pf c_pf)
           (WF_J: wf_j views c_j)
+          (WF_APF: wf_ra rels c_apf)
           (WF_RA: wf_ra rels c_ra)
-          (RACEFREE: RARaceW.racefree L rels c_ra):
-      behaviors (PFConfiguration.machine_step L) c_pf <1=
-      behaviors (@OrdConfiguration.machine_step L Ordering.acqrel) c_ra.
+          (RACEFREE: RARaceW.racefree L Ordering.acqrel Ordering.acqrel rels c_ra):
+      behaviors (PFConfiguration.machine_step L) c_pf <2=
+      behaviors (@OrdConfiguration.machine_step L Ordering.acqrel Ordering.acqrel) c_ra.
     Proof.
-      i. revert views rels c_j c_ra SIM WF_PF WF_J WF_RA RACEFREE.
+      i. revert views rels c_j c_apf c_ra SIM WF_PF WF_J WF_APF WF_RA RACEFREE.
       induction PR; i.
       - econs 1. eapply sim_conf_terminal; eauto.
       - inv STEP. exploit sim_conf_step; eauto. i. des.
         + exploit RARaceW.step_ord_step; eauto. i.
-          inv EVENT_J; inv EVENT_RA; ss. inv H0.
+          inv EVENT_J; inv EVENT_APF; inv EVENT_RA; ss. inv H0.
           econs 2.
-          { replace (MachineEvent.syscall e) with
-                (ThreadEvent.get_machine_event (ThreadEvent.syscall e)) by ss.
-            econs; eauto. }
-          hexploit RARaceW.step_racefree; eauto. i.
-          exploit step_pf_future; eauto. i. des.
-          exploit step_j_future; eauto. i. des.
-          exploit step_ra_future; eauto.
-        + exfalso. unfold RARaceW.ra_race_steps in *. des. eauto.
-      - inv STEP. exploit sim_conf_step; eauto. i. des.
-        + exploit RARaceW.step_ord_step; eauto. i.
-          inv EVENT_J; inv EVENT_RA; ss. inv H0.
-          econs 3.
-          replace MachineEvent.failure with (ThreadEvent.get_machine_event ThreadEvent.failure) by ss.
-          econs; eauto.
-        + exfalso. unfold RARaceW.ra_race_steps in *. des. eauto.
-      - inv STEP. exploit sim_conf_step; eauto. i. des.
-        + exploit RARaceW.step_ord_step; eauto. i.
-          econs 4.
-          { replace MachineEvent.silent with (ThreadEvent.get_machine_event e_ra); cycle 1.
-            { inv EVENT_J; inv EVENT_RA; ss. }
+          { replace (MachineEvent.syscall e2) with
+                (ThreadEvent.get_machine_event (ThreadEvent.syscall e2)) by ss.
             econs; eauto.
           }
           hexploit RARaceW.step_racefree; eauto. i.
           exploit step_pf_future; eauto. i. des.
           exploit step_j_future; eauto. i. des.
-          exploit step_ra_future; eauto.
+          exploit step_ra_future; try exact STEP_APF; eauto. i. des.
+          exploit step_ra_future; try exact STEP_RA; eauto. ss.
         + exfalso. unfold RARaceW.ra_race_steps in *. des. eauto.
+      - inv STEP. exploit sim_conf_step; eauto. i. des.
+        + exploit RARaceW.step_ord_step; eauto. i.
+          econs 3.
+          replace MachineEvent.failure with (ThreadEvent.get_machine_event e_ra); [econs; eauto|].
+          inv EVENT_J; inv EVENT_APF; inv EVENT_RA; ss.
+        + exfalso. unfold RARaceW.ra_race_steps in *. des. eauto.
+      - inv STEP. exploit sim_conf_step; eauto. i. des.
+        + exploit RARaceW.step_ord_step; eauto. i.
+          econs 4.
+          { replace MachineEvent.silent with (ThreadEvent.get_machine_event e_ra); cycle 1.
+            { inv EVENT_J; inv EVENT_APF; inv EVENT_RA; ss. }
+            econs; eauto.
+          }
+          hexploit RARaceW.step_racefree; eauto. i.
+          exploit step_pf_future; eauto. i. des.
+          exploit step_j_future; eauto. i. des.
+          exploit step_ra_future; try exact STEP_APF; eauto. i. des.
+          exploit step_ra_future; try exact STEP_RA; eauto.
+        + exfalso. unfold RARaceW.ra_race_steps in *. des. eauto.
+      - econs 5.
     Qed.
   End PFtoRA.
 End PFtoRA.
